src/ecDecl.mli
@@ -235,6 +235,7 @@ type bv_opkind = [
   | `Extend   of int * int * bool (* size in + size out + sign *)
   | `Truncate of int * int (* size in + size out *)
   | `Extract  of int * int (* size in + size out *)
+  | `Insert   of int * int (* size in + size out *)
   | `Concat   of int * int * int (* size in1 + size in2 + size out *)
   | `Init     of int (* size_out *)
   | `Get      of int (* size_in *)
